Initial scaffolding Recombination proofs
Following Composition and generalizing the mergeability relation to
expose interface information. It ends up being more verbose than its PS
counterpart, principally due to the involvement of two explicit pairs of
programs.

Sectioning and greedy inclusion of hypotheses in admitted lemmas make
some of the later proofs break until the now external hypotheses are
named explicitly, to be fixed when it is clear the high-level structure
continues to work, as expected.

Intermediate/Recombination.v
@@ -31,6 +31,33 @@ Import Intermediate.
    to those modules can be added here. Note that, in principle, the role of PS
    will be assimilated by Recombination or become very reduced. *)
 
+(* An "extensional" reading of program states a la Composition.
+   RB: TODO: If the number, organization and order of parameters is confusing,
+   look at alternatives, here and in the sections that use this. *)
+Inductive mergeable_states (ic ip : Program.interface) (s s'' : CS.state)
+  : Prop :=
+  mergeable_states_intro : forall p c p' c' s0 s0'' t,
+    mergeable_interfaces ip ic ->
+    prog_interface p = ip ->
+    prog_interface c = ic ->
+    prog_interface p' = ip ->
+    prog_interface c' = ic ->
+    initial_state (CS.sem (program_link p  c )) s0   ->
+    initial_state (CS.sem (program_link p' c')) s0'' ->
+    Star (CS.sem (program_link p  c )) s0   t s   ->
+    Star (CS.sem (program_link p' c')) s0'' t s'' ->
+    mergeable_states ic ip s s''.
+
+Definition merge_states (s s'' : CS.state) : CS.state :=
+  s.
+
+Lemma mergeable_states_context_to_program ctx1 ctx2 s1 s2 :
+  mergeable_states ctx1 ctx2 s1 s2 ->
+  CS.is_context_component s1 ctx1 ->
+  CS.is_program_component s2 ctx2.
+Admitted.
+
+
 Section BehaviorStar.
   Variables p c: program.
 
@@ -116,6 +143,84 @@ Section BehaviorStar.
   Qed.
 End BehaviorStar.
 
+Section ThreewayMultisemProgram.
+  Variables p c p' c' : program.
+
+  Hypothesis Hwfp  : well_formed_program p.
+  Hypothesis Hwfc  : well_formed_program c.
+  Hypothesis Hwfp' : well_formed_program p'.
+  Hypothesis Hwfc' : well_formed_program c'.
+
+  Hypothesis Hmergeable_ifaces :
+    mergeable_interfaces (prog_interface p) (prog_interface c).
+
+  Hypothesis Hifacep  : prog_interface p  = prog_interface p'.
+  Hypothesis Hifacec  : prog_interface c  = prog_interface c'.
+
+  (* RB: TODO: Simplify redundancies in standard hypotheses. *)
+  Hypothesis Hmain_linkability  : linkable_mains p  c.
+  Hypothesis Hmain_linkability' : linkable_mains p' c'.
+
+  Hypothesis Hprog_is_closed  : closed_program (program_link p  c ).
+  Hypothesis Hprog_is_closed' : closed_program (program_link p' c').
+
+  Theorem threeway_multisem_mergeable_program s1 s1'' t s2 s2'' :
+    CS.is_program_component s1 (prog_interface c) ->
+    mergeable_states (prog_interface c) (prog_interface p) s1 s1'' ->
+    Star (CS.sem (program_link p  c )) s1   t s2   ->
+    Star (CS.sem (program_link p' c')) s1'' t s2'' ->
+    mergeable_states (prog_interface c) (prog_interface p) s2 s2''.
+  Admitted.
+
+  Theorem threeway_multisem_star_program s1 s1'' t s2 s2'' :
+    CS.is_program_component s1 (prog_interface c) ->
+    mergeable_states (prog_interface c) (prog_interface p) s1 s1'' ->
+    Star (CS.sem (program_link p  c )) s1   t s2   ->
+    Star (CS.sem (program_link p' c')) s1'' t s2'' ->
+    Star (CS.sem (program_link p  c')) (merge_states s1 s1'') t (merge_states s2 s2'').
+  Admitted.
+End ThreewayMultisemProgram.
+
+Section ThreewayMultisem.
+  Variables p c p' c' : program.
+
+  Hypothesis Hwfp  : well_formed_program p.
+  Hypothesis Hwfc  : well_formed_program c.
+  Hypothesis Hwfp' : well_formed_program p'.
+  Hypothesis Hwfc' : well_formed_program c'.
+
+  Hypothesis Hmergeable_ifaces :
+    mergeable_interfaces (prog_interface p) (prog_interface c).
+
+  Hypothesis Hifacep  : prog_interface p  = prog_interface p'.
+  Hypothesis Hifacec  : prog_interface c  = prog_interface c'.
+
+  (* RB: TODO: Simplify redundancies in standard hypotheses. *)
+  Hypothesis Hmain_linkability  : linkable_mains p  c.
+  Hypothesis Hmain_linkability' : linkable_mains p' c'.
+
+  Hypothesis Hprog_is_closed  : closed_program (program_link p  c ).
+  Hypothesis Hprog_is_closed' : closed_program (program_link p' c').
+
+  (* RB: NOTE: At the moment, this becomes the old threeway_multisem_star. *)
+  Theorem threeway_multisem_star_simulation s1 s1'' t s2 s2'' :
+    mergeable_states (prog_interface c) (prog_interface p) s1 s1'' ->
+    Star (CS.sem (program_link p  c )) s1   t s2   ->
+    Star (CS.sem (program_link p' c')) s1'' t s2'' ->
+    Star (CS.sem (program_link p  c')) (merge_states s1 s1'') t (merge_states s2 s2'').
+    (* /\ mergeable_states ip ic s2 s2'' *)
+  Proof.
+    intros Hmerge1 Hstar12 Hstar12''.
+    destruct (CS.is_program_component s1 (prog_interface c)) eqn:Hcomp1.
+    - now apply threeway_multisem_star_program.
+    - apply negb_false_iff in Hcomp1.
+      apply (mergeable_states_context_to_program Hmerge1) in Hcomp1.
+      rewrite program_linkC; try assumption;
+        last admit.
+      apply threeway_multisem_star_program with (c := p') (p' := c).
+  Admitted.
+End ThreewayMultisem.
+
 Section Recombination.
   Variables p c p' c' : program.
 
@@ -137,36 +242,18 @@ Section Recombination.
   Hypothesis Hprog_is_closed  : closed_program (program_link p  c ).
   Hypothesis Hprog_is_closed' : closed_program (program_link p' c').
 
-  (* An "extensional" reading of program states a la Composition. *)
-  Inductive mergeable_states (s s'' : CS.state) : Prop :=
-    mergeable_states_intro : forall s0 s0'' t,
-      initial_state (CS.sem (program_link p  c )) s0   ->
-      initial_state (CS.sem (program_link p' c')) s0'' ->
-      Star (CS.sem (program_link p  c )) s0   t s   ->
-      Star (CS.sem (program_link p' c')) s0'' t s'' ->
-      mergeable_states s s''.
-
-  Definition merge_states (s s'' : CS.state) : CS.state :=
-    s.
-
+  (* RB: NOTE: Relocate lemmas on initial states when ready. *)
   Theorem initial_states_mergeability s s'' :
     initial_state (CS.sem (program_link p  c )) s   ->
     initial_state (CS.sem (program_link p' c')) s'' ->
-    mergeable_states s s''.
+    mergeable_states (prog_interface c) (prog_interface p) s s''.
   Admitted.
 
+  (* RB: NOTE: Relocate lemmas on initial states when ready. *)
   Lemma initial_state_merge_after_linking s s'' :
     initial_state (CS.sem (program_link p  c )) s   ->
     initial_state (CS.sem (program_link p' c')) s'' ->
     initial_state (CS.sem (program_link p  c')) (merge_states s s'').
-  Admitted.
-
-  Theorem threeway_multisem_star_simulation s1 s1'' t s2 s2'' :
-    mergeable_states s1 s1'' ->
-    Star (CS.sem (program_link p  c )) s1   t s2   ->
-    Star (CS.sem (program_link p' c')) s1'' t s2'' ->
-    Star (CS.sem (program_link p  c')) (merge_states s1 s1'') t (merge_states s2 s2'').
-    (* /\ mergeable_states ip ic s2 s2'' *)
   Admitted.
 
   (* RB: NOTE: Possible improvements:
